examples/lowparse/LowParse.Impl.Array.fst
@@ -1,0 +1,35 @@
+module LowParse.Impl.Array
+include LowParse.Impl.FLBytes
+include LowParse.Impl.Seq
+include LowParse.Spec.Array
+
+module U32 = FStar.UInt32
+module S = LowParse.Slice
+
+inline_for_extraction
+val validate_array_gen
+  (#elem_byte_size: nat)
+  (#k: constant_size_parser_kind)
+  (#t: Type0)
+  (#p: parser (ParserStrong (StrongConstantSize elem_byte_size k)) t)
+  (vs: stateful_validator p)
+  (array_byte_size: U32.t)
+  (precond: squash (array_type_of_parser_kind_precond elem_byte_size (U32.v array_byte_size)))
+: Tot (stateful_validator (parse_array p (U32.v array_byte_size) precond))
+
+let validate_array_gen #elem_byte_size #k #t #p vs array_byte_size precond =
+  fun (s: S.bslice) -> validate_flbytes (validate_seq vs) array_byte_size s
+
+inline_for_extraction
+let validate_array
+  (#elem_byte_size: nat)
+  (#k: constant_size_parser_kind)
+  (#t: Type0)
+  (#p: parser (ParserStrong (StrongConstantSize elem_byte_size k)) t)
+  (vs: stateful_validator p)
+  (array_byte_size: U32.t)
+  (precond: squash (array_type_of_parser_kind_precond elem_byte_size (U32.v array_byte_size)))
+: Tot (stateful_validator (parse_array p (U32.v array_byte_size) precond))
+= if ConstantSizeTotal? k
+  then validate_total_constant_size array_byte_size (parse_array p (U32.v array_byte_size) precond)
+  else validate_array_gen vs array_byte_size precond
