examples/lowparse/LowParse.Spec.Array.fst
@@ -1,0 +1,175 @@
+module LowParse.Spec.Array
+include LowParse.Spec.FLBytes
+include LowParse.Spec.Seq
+
+module Seq = FStar.Seq
+module PL = LowParse.Spec.List
+
+type array (t: Type) (n: nat) = (s: Seq.seq t { Seq.length s == n } )
+
+let array_type_of_parser_kind_precond (elem_byte_size: nat) (array_byte_size: nat) : GTot bool =
+  elem_byte_size > 0 &&
+  array_byte_size % elem_byte_size = 0
+
+let array_type_of_parser
+  (#elem_byte_size: nat)
+  (#k: constant_size_parser_kind)
+  (#t: Type0)
+  (p: parser (ParserStrong (StrongConstantSize elem_byte_size k)) t)
+  (array_byte_size: nat)
+: Pure Type0
+  (requires (
+    array_type_of_parser_kind_precond elem_byte_size array_byte_size
+  ))
+  (ensures (fun _ -> True))
+= array t (array_byte_size / elem_byte_size)
+
+val parse_array_correct
+  (#elem_byte_size: nat)
+  (#k: constant_size_parser_kind)
+  (#t: Type0)
+  (p: parser (ParserStrong (StrongConstantSize elem_byte_size k)) t)
+  (array_byte_size: nat)
+  (b: bytes32)
+: Lemma
+  (requires (
+    array_type_of_parser_kind_precond elem_byte_size array_byte_size /\
+    Some? (parse (parse_flbytes (parse_seq p) array_byte_size) b)
+  ))
+  (ensures (
+    array_type_of_parser_kind_precond elem_byte_size array_byte_size /\ (
+    let pb = parse (parse_flbytes (parse_seq p) array_byte_size) b in
+    Some? pb /\ (
+    let (Some (data, _)) = pb in
+    Seq.length data == array_byte_size / elem_byte_size
+  ))))
+
+let parse_array_correct #elem_byte_size #k #t p array_byte_size b =
+  let (Some (data, consumed)) = parse (parse_flbytes (parse_seq p) array_byte_size) b in
+  assert (consumed == array_byte_size);
+  let b' = Seq.slice b 0 consumed in
+  seq_length_constant_size_parser_correct p b';
+  FStar.Math.Lemmas.multiple_division_lemma (Seq.length data) elem_byte_size
+
+let parse_array'
+  (#elem_byte_size: nat)
+  (#k: constant_size_parser_kind)
+  (#t: Type0)
+  (p: parser (ParserStrong (StrongConstantSize elem_byte_size k)) t)
+  (array_byte_size: nat)
+  (precond: squash (array_type_of_parser_kind_precond elem_byte_size array_byte_size))
+: Tot (bare_parser (array_type_of_parser p array_byte_size))
+= fun (b: bytes32) ->
+  match parse (parse_flbytes (parse_seq p) array_byte_size) b with
+  | None -> None
+  | Some (data, consumed) ->
+    parse_array_correct p array_byte_size b;
+    let data' : array t (array_byte_size / elem_byte_size) = data in
+    Some (data' , consumed)
+
+let parse_array_injective
+  (#elem_byte_size: nat)
+  (#k: constant_size_parser_kind)
+  (#t: Type0)
+  (p: parser (ParserStrong (StrongConstantSize elem_byte_size k)) t)
+  (array_byte_size: nat)
+  (precond: squash (array_type_of_parser_kind_precond elem_byte_size array_byte_size))
+: Lemma
+  (injective (parse_array' p array_byte_size precond))
+= let p' : bare_parser (array_type_of_parser p array_byte_size) = parse_array' p array_byte_size precond in
+  let prf
+    (b1 b2: bytes32)
+  : Lemma
+    (requires (injective_precond p' b1 b2))
+    (ensures (injective_postcond p' b1 b2))
+  = assert (injective_postcond (parse_flbytes (parse_seq p) array_byte_size) b1 b2)
+  in
+  let prf'
+    (b1 b2: bytes32)
+  : Lemma
+    (injective_precond p' b1 b2 ==> injective_postcond p' b1 b2)
+  = Classical.move_requires (prf b1) b2
+  in
+  Classical.forall_intro_2 prf'
+
+val parse_total_constant_size_elem_parse_list_total
+  (#elem_byte_size: nat)
+  (#t: Type0)
+  (p: parser (ParserStrong (StrongConstantSize elem_byte_size ConstantSizeTotal)) t)
+  (array_byte_size: nat)
+  (b: bytes32)
+: Lemma
+  (requires (
+    array_type_of_parser_kind_precond elem_byte_size array_byte_size /\
+    Seq.length b % elem_byte_size == 0
+  ))
+  (ensures (
+    Some? (parse (PL.parse_list p) b)
+  ))
+  (decreases (Seq.length b))
+
+let rec parse_total_constant_size_elem_parse_list_total #elem_byte_size #t p array_byte_size b =
+  if Seq.length b = 0
+  then ()
+  else begin
+    assert (Seq.length b >= elem_byte_size);
+    let pe = parse p b in
+    assert (Some? pe);
+    let (Some (_, consumed)) = pe in
+    assert ((consumed <: nat) == elem_byte_size);
+    let b' = Seq.slice b consumed (Seq.length b) in
+    FStar.Math.Lemmas.lemma_mod_plus (Seq.length b') 1 elem_byte_size;
+    parse_total_constant_size_elem_parse_list_total p array_byte_size b' ;    
+    assume (Some? (parse (PL.parse_list p) b))
+  end
+
+val parse_total_constant_size_elem_parse_array_total'
+  (#elem_byte_size: nat)
+  (#t: Type0)
+  (p: parser (ParserStrong (StrongConstantSize elem_byte_size ConstantSizeTotal)) t)
+  (array_byte_size: nat)
+  (precond: squash (array_type_of_parser_kind_precond elem_byte_size array_byte_size))
+  (b: bytes32)
+: Lemma
+  (requires (
+    Seq.length b >= array_byte_size
+  ))
+  (ensures (
+    Some? (parse (parse_array' p array_byte_size precond) b)
+  ))
+
+let parse_total_constant_size_elem_parse_array_total' #elem_byte_size #t p array_byte_size precond b =
+  let b' = Seq.slice b 0 array_byte_size in
+  parse_total_constant_size_elem_parse_list_total p array_byte_size b';
+  parse_seq_correct p b'
+
+let parse_total_constant_size_elem_parse_array_total
+  (#elem_byte_size: nat)
+  (#k: constant_size_parser_kind)
+  (#t: Type0)
+  (p: parser (ParserStrong (StrongConstantSize elem_byte_size k)) t)
+  (array_byte_size: nat)
+  (precond: squash (array_type_of_parser_kind_precond elem_byte_size array_byte_size))
+: Lemma
+  (ensures (
+    ConstantSizeTotal? k ==> (forall (b: bytes32) .
+    Seq.length b >= array_byte_size ==>
+    Some? (parse (parse_array' p array_byte_size precond) b)
+  )))
+= if ConstantSizeTotal? k
+  then
+    let p' : parser (ParserStrong (StrongConstantSize elem_byte_size ConstantSizeTotal)) t = p in
+    Classical.forall_intro (Classical.move_requires (parse_total_constant_size_elem_parse_array_total' p' array_byte_size ()))
+  else ()
+
+let parse_array
+  (#elem_byte_size: nat)
+  (#k: constant_size_parser_kind)
+  (#t: Type0)
+  (p: parser (ParserStrong (StrongConstantSize elem_byte_size k)) t)
+  (array_byte_size: nat)
+  (precond: squash (array_type_of_parser_kind_precond elem_byte_size array_byte_size))
+: Tot (parser (ParserStrong (StrongConstantSize array_byte_size k)) (array_type_of_parser p array_byte_size))
+= parse_array_injective p array_byte_size precond;
+  parse_total_constant_size_elem_parse_array_total p array_byte_size precond;
+  parse_array' p array_byte_size precond
